completeness progress

Hybrid/Form.lean
@@ -1,5 +1,8 @@
 import Mathlib.Data.Set.Basic
-import Mathlib.Data.Nat.Parity
+import Mathlib.Data.List.Sort
+import Mathlib.Data.List.Lemmas
+import Mathlib.Data.Fin.Basic
+import Mathlib.Logic.Equiv.Fin
 import Hybrid.Util
 
 section Basics
@@ -22,9 +25,18 @@ section Basics
   instance : Max NOM where
     max := λ i => λ j => ite (i.letter > j.letter) i j
 
+  theorem NOM_eq {i j : NOM} : (i = j) ↔ (i.letter = j.letter) := by
+    cases i
+    cases j
+    simp
+  theorem NOM_eq' {i j : NOM} : (i = j) ↔ (j.letter = i.letter) := by
+    cases i
+    cases j
+    simp
+    apply Iff.intro <;> {intro; simp [*]}
 
-  instance : OfNat SVAR n    where
-    ofNat := SVAR.mk n
+--  instance ofNatSVAR : OfNat SVAR n    where
+--    ofNat := SVAR.mk n
   instance : OfNat NOM n     where
     ofNat := NOM.mk  n
   instance : Coe SVAR Nat  := ⟨SVAR.letter⟩
@@ -33,20 +45,34 @@ section Basics
 --  instance : Coe Nat NOM   := ⟨NOM.mk⟩   
   instance SVAR.le : LE SVAR         where
     le    := λ x => λ y =>  x.letter ≤ y.letter
-  instance : LT SVAR         where
+  instance SVAR.lt : LT SVAR         where
     lt    := λ x => λ y =>  x.letter < y.letter
   instance NOM.le : LE NOM         where
     le    := λ x => λ y =>  x.letter ≤ y.letter
-  instance  : HAdd SVAR Nat SVAR where
+  instance NOM.lt : LT NOM         where
+    lt    := λ x => λ y =>  x.letter < y.letter
+  instance SVAR.add : HAdd SVAR Nat SVAR where
     hAdd  := λ x => λ n => SVAR.mk (x.letter + n)
-  instance : HAdd NOM Nat NOM where
+  instance NOM.add : HAdd NOM Nat NOM where
     hAdd  := λ x => λ n => NOM.mk (x.letter + n)
   instance : HMul NOM Nat NOM where
     hMul  := λ x => λ n => NOM.mk (x.letter * n)
-  instance : HMul Nat NOM NOM where
+  instance NOM.hmul : HMul Nat NOM NOM where
     hMul  := λ n => λ x => NOM.mk (x.letter * n)
   instance : HMul NOM ℕ ℕ where
     hMul  := λ x => λ n => x.letter * n
+
+  instance : IsTrans NOM GT.gt where
+    trans := λ _ _ _ h1 h2 => Nat.lt_trans h2 h1
+
+  instance : IsTotal NOM GE.ge where
+    total := by simp [NOM.le, Nat.le_total]
+
+  instance : IsTrans NOM GE.ge where
+    trans := λ _ _ _ h1 h2 => Nat.le_trans h2 h1
+
+  theorem NOM.gt_iff_ge_and_ne {a b : NOM} : a > b ↔ (a ≥ b ∧ a ≠ b) := by
+    simp only [GT.gt, GE.ge, NOM.lt, NOM.le, NOM.mk, Nat.lt_iff_le_and_ne, ne_eq, NOM_eq']
 
   inductive Form where
     -- atomic formulas:
@@ -61,6 +87,12 @@ section Basics
     -- hybrid:
     | bind : SVAR → Form → Form
   deriving DecidableEq, Repr
+
+  def Form.depth : Form → ℕ
+    | .impl φ ψ =>  1 + Form.depth φ + Form.depth ψ
+    | .box  φ   =>  1 + Form.depth φ
+    | .bind _ φ =>  2 + Form.depth φ
+    | _       =>    0
 
   @[simp]
   def Form.neg      : Form → Form := λ φ => Form.impl φ Form.bttm
@@ -100,14 +132,14 @@ section Basics
   | .impl ψ χ => max (ψ.new_var) (χ.new_var)
   | .box  ψ   => ψ.new_var
   | .bind x ψ => max (x+1) (ψ.new_var)
-  | _         => 0
+  | _         => ⟨0⟩
 
   def Form.new_nom  : Form → NOM
   | .nom  i   => i+1
   | .impl ψ χ => max (ψ.new_nom) (χ.new_nom)
   | .box  ψ   => ψ.new_nom
   | .bind _ ψ => ψ.new_nom
-  | _         => 0
+  | _         => ⟨0⟩ 
 
 end Basics
 
@@ -131,9 +163,6 @@ section Substitutions
     | Form.impl φ ψ => (is_free x φ) || (is_free x ψ)
     | Form.box  φ   => is_free x φ
     | Form.bind y φ => (y != x) && (is_free x φ)
-
-  #eval is_free (SVAR.mk 0) ⊥
-  #eval is_free (SVAR.mk 0) (all SVAR.mk 0, ⊥)
 
   def is_bound (x : SVAR) (φ : Form) := (occurs x φ) && !(is_free x φ)
   
@@ -183,238 +212,9 @@ section Substitutions
   notation:150 φ "[" s "//" x "]" => subst_svar φ s x
   notation:150 φ "[" s "//" x "]" => subst_nom  φ s x
 
-  #eval is_substable (all SVAR.mk 0, all SVAR.mk 1, SVAR.mk 0) (SVAR.mk 1) (SVAR.mk 0)  
-  #eval subst_svar (all SVAR.mk 0, all SVAR.mk 1, SVAR.mk 0) (SVAR.mk 1) (SVAR.mk 0)
-  #eval occurs 1 (all 0, all 1, SVAR.mk 0)
-
-  lemma new_var_gt      : occurs x φ → x < φ.new_var   := by
-    induction φ with
-    | svar y          =>
-        simp [occurs, Form.new_var, -implication_disjunction]
-        intro h
-        rw [h]
-        exact Nat.lt_succ_self y.letter
-    | impl ψ χ ih1 ih2 =>
-        simp only [occurs, Form.new_var, Bool.or_eq_true, max]
-        intro h
-        apply Or.elim h
-        . intro ha
-          clear ih2 h
-          have ih1 := ih1 ha
-          by_cases hc : (Form.new_var ψ).letter > (Form.new_var χ).letter
-          . simp [hc]
-            assumption
-          . simp [hc]
-            simp at hc 
-            exact Nat.lt_of_lt_of_le ih1 hc
-        . intro hb
-          clear ih1 h
-          have ih2 := ih2 hb
-          by_cases hc : (Form.new_var ψ).letter > (Form.new_var χ).letter
-          . simp [hc]
-            simp at hc
-            exact Nat.lt_trans ih2 hc
-          . simp [hc]
-            assumption
-    | box ψ ih      =>
-        simp only [occurs, Form.new_var]
-        assumption
-    | bind y ψ ih   =>
-        simp only [occurs, Form.new_var, max]
-        intro h
-        have ih := ih h
-        by_cases hc : (y + 1).letter > (Form.new_var ψ).letter
-        . simp [hc]
-          simp at hc
-          exact Nat.lt_trans ih hc
-        . simp [hc]
-          assumption
-    | _ => simp [occurs]
-
-  lemma new_var_is_new  : occurs (φ.new_var) φ = false := by
-    rw [←Bool.eq_false_eq_not_eq_true]
-    intro h
-    have a := new_var_gt h
-    have b := Nat.lt_irrefl φ.new_var.letter
-    exact b a
-  
-  lemma ge_new_var_is_new (h : x ≥ φ.new_var) : occurs x φ = false := by
-    rw [←Bool.eq_false_eq_not_eq_true]
-    intro habs
-    have := new_var_gt habs
-    have a := Nat.lt_of_le_of_lt h this
-    have b := Nat.lt_irrefl φ.new_var.letter
-    exact b a
-  
-  lemma notfreeset {Γ : Set Form} (L : List Γ) (hyp : ∀ ψ : Γ, is_free x ψ = false) : is_free x (conjunction Γ L) = false := by
-    induction L with
-    | nil         =>
-        simp only [conjunction, is_free]
-    | cons h t ih =>
-        simp only [is_free, Bool.or_false, Bool.or_eq_false_eq_eq_false_and_eq_false]
-        apply And.intro
-        . exact hyp h
-        . exact ih
-
-  lemma notfree_after_subst {φ : Form} {x y : SVAR} (h : x ≠ y) : is_free x (φ[y // x]) = false := by
-    induction φ with
-    | svar z   =>
-        by_cases xz : x = z
-        . simp [subst_svar, if_pos xz, is_free, h]
-        . simp [subst_svar, if_neg xz, is_free, xz]
-    | impl _ _ ih1 ih2 =>
-        simp [subst_svar, is_free, ih1, ih2]
-    | box _ ih    =>
-        simp [subst_svar, is_free, ih]
-    | bind z _ ih =>
-        by_cases xz : x = z
-        . simp [subst_svar, xz, is_free]
-        . simp [subst_svar, if_neg xz, is_free, ih]
-    | _        => simp only [is_free]
-
-  lemma notocc_beforeafter_subst {φ : Form} {x y : SVAR} (h : occurs x φ = false) : occurs x (φ[y // x]) = false := by
-    induction φ with
-    | svar z   =>
-        by_cases xz : x = z
-        <;> simp [subst_svar, if_pos xz, xz, occurs, h] at *
-    | impl _ _ ih1 ih2 =>
-        simp [subst_svar, occurs, not_or, ih1, ih2, -implication_disjunction] at *
-        exact ⟨ih1 h.left, ih2 h.right⟩ 
-    | box _ ih    =>
-        simp [subst_svar, occurs, ih, -implication_disjunction] at *
-        exact ih h
-    | bind z ψ ih =>
-        by_cases xz : x = z
-        . simp [subst_svar, xz, occurs] at *
-          exact h
-        . simp [subst_svar, if_neg xz, occurs, ih, xz, h, -implication_disjunction] at *
-          exact ih h
-    | _        => simp only [occurs]
-
-  lemma notoccursbind : occurs x φ = false → occurs x (all v, φ) = false := by
-    simp [occurs]
-
-  lemma notoccurs_notfree : (occurs x φ = false) → (is_free x φ = false) := by
-    induction φ with
-    | svar _ => simp [occurs, is_free]
-    | impl _ _ ih1 ih2 =>
-        intro h
-        simp [occurs] at h
-        simp [is_free, ih1, ih2, h]
-    | box _ ih        =>
-        intro h
-        rw [occurs] at h
-        simp [is_free, ih, h]
-    | bind _ _ ih     =>
-        intro h
-        rw [occurs] at h
-        simp [is_free, ih, h]
-    | _ => 
-        intro h
-        rfl
-
-  lemma preserve_notfree {φ : Form} (x v : SVAR) : (is_free x φ = false) → (is_free x (all v, φ) = false) := by
-    intro h
-    simp only [is_free, h, Bool.and_false]
-
-  -- φ = all x, all y, x
-  -- φ[y // x] = φ:                 (x is bound in φ)
-  #eval (all SVAR.mk 0, all SVAR.mk 1, SVAR.mk 0)[SVAR.mk 1 // SVAR.mk 0]
-  --  but is_subst φ y x = false:   (x occurs free in the scope of y)
-  #eval is_substable (all SVAR.mk 0, all SVAR.mk 1, SVAR.mk 0) (SVAR.mk 1) (SVAR.mk 0)
-  lemma subst_notfree_var {φ : Form} {x y : SVAR} (h : is_free x φ = false) : (φ[y // x] = φ) ∧ (occurs x φ = false → is_substable φ y x) := by
-    induction φ with
-    | svar z =>
-        by_cases heq : x = z
-        . simp only [is_free, heq, beq_self_eq_true] at h 
-        . simp only [subst_svar, heq, ite_false, occurs, is_substable]
-    | impl ψ χ ih1 ih2 =>
-        simp only [is_free, Bool.or_eq_false_eq_eq_false_and_eq_false] at h 
-        apply And.intro
-        . simp [subst_svar, h, ih1, ih2]
-        . intro nocc
-          simp only [occurs, Bool.or_eq_false_eq_eq_false_and_eq_false] at nocc 
-          simp [is_substable, h, nocc, ih1, ih2]
-    | box ψ ih  =>
-        rw [is_free] at h
-        apply And.intro
-        . simp [subst_svar, ih, h]
-        . intro nocc
-          rw [occurs] at nocc
-          simp [is_substable, ih, nocc, h]
-    | bind z ψ ih =>
-        apply And.intro
-        . by_cases heq : x = z
-          . rw [←heq, subst_svar, if_pos (Eq.refl x)]
-          . simp only [is_free, bne, Bool.and_eq_false_eq_eq_false_or_eq_false, Bool.not_eq_false', beq_iff_eq,
-            Ne.symm heq, false_or] at h 
-            simp [subst_svar, heq, ih, h]
-        . intro nocc
-          rw [occurs] at nocc
-          simp [is_substable, notoccurs_notfree, nocc]
-    | _   =>
-        simp [subst_svar, is_substable]
-
-    lemma rereplacement (φ : Form) (x y : SVAR) (h1 : occurs y φ = false) (h2 : is_substable φ y x) : (is_substable (φ[y // x]) x y) ∧ φ[y // x][x // y] = φ := by
-      induction φ with
-      | svar z =>
-          simp [occurs] at h1
-          by_cases xz : x = z
-          repeat simp [subst_svar, xz, h1, is_substable]
-      | impl ψ χ ih1 ih2 =>
-          simp only [occurs, Bool.or_eq_false_eq_eq_false_and_eq_false] at h1 
-          simp only [is_substable, Bool.and_eq_true] at h2
-          simp [subst_svar, ih1, ih2, h1, h2, is_substable]
-      | box ψ ih =>
-          simp only [occurs] at h1
-          simp only [is_substable] at h2
-          simp [subst_svar, ih, h1, h2, is_substable]
-      | bind z ψ ih =>
-          by_cases yz : y = z
-          . rw [←yz]
-            rw [←yz] at h1
-
-            simp only [is_substable, beq_iff_eq, ←yz, bne_self_eq_false, Bool.false_and, ite_eq_left_iff,
-              Bool.not_eq_false, implication_disjunction, Bool.not_eq_true, or_false] at h2 
-            have h2 := @preserve_notfree ψ x y h2
-            simp [subst_notfree_var, h2]
-
-            have := @subst_notfree_var (all y, ψ) y x (notoccurs_notfree h1)
-            simp [@subst_notfree_var (all y, ψ) y x, notoccurs_notfree, h1]
-          . by_cases xz : x = z
-            . have : is_free x (all x, ψ) = false := by simp [is_free]
-              rw [←xz] at h1
-              simp [←xz, subst_notfree_var, this, notoccurs_notfree, h1]
-            . simp only [occurs] at h1
-              simp [subst_svar, xz, yz]
-              by_cases xfree : is_free x ψ
-              . simp [is_substable, xfree, Ne.symm yz, bne] at h2
-                simp [ih, h1, h2, is_substable, bne, Ne.symm xz]
-              . rw [show (¬is_free x ψ = true ↔ is_free x ψ = false) by simp] at xfree
-                simp [subst_notfree_var, xfree, is_substable, (notoccurs_notfree h1)]
-      | _     =>
-          apply And.intro
-          repeat rfl
-  
-  lemma subst_self_is_self (φ : Form) (x : SVAR) : φ [x // x] = φ := by
-    induction φ with
-    | svar y   =>
-        by_cases xy : x = y
-        . rw [subst_svar, if_pos xy, xy]
-        . rw [subst_svar, if_neg xy]
-    | impl φ ψ ih1 ih2 =>
-        rw [subst_svar, ih1, ih2]
-    | box  φ ih  =>
-        rw [subst_svar, ih]
-    | bind y φ ih =>
-        by_cases xy : x = y
-        . rw [subst_svar, if_pos xy]
-        . rw [subst_svar, if_neg xy, ih]
-    | _        => rfl
-
 end Substitutions
 
-section NominalSubstitution
+section NominalSubstitution 
 
   def Form.nominals : Form → List NOM
   | .nom a      => [a]
@@ -447,401 +247,57 @@ section NominalSubstitution
   | i, .bind _ ψ => nom_occurs i ψ
   | _, _         => false
 
-  def Form.list_noms : Form → List NOM := λ φ =>
-    loop φ.new_nom.letter φ
-  where
-    loop : Nat → Form → List NOM
-    | 0, _     =>      []
-    | n+1, φ   => ite (nom_occurs ⟨n⟩ φ) (⟨n⟩ :: loop n φ) (loop n φ)
+  def all_nocc (i : NOM) (Γ : Set Form) := ∀ (φ : Form), φ ∈ Γ → nom_occurs i φ = false
 
-  def Form.dbl_list_noms : Form → List NOM := λ φ =>
-    loop φ.new_nom.letter φ
-  where
-    loop : Nat → Form → List NOM
-    | 0, _     =>      []
-    | n+1, φ   =>      ite (nom_occurs ⟨n⟩ φ) (⟨2*n⟩ :: loop n φ) (loop n φ)
-  
-  #eval (NOM.mk 2 ⋁ NOM.mk 3 ⋁ NOM.mk 4).list_noms
-  #eval List.take 9 (NOM.mk 2 ⋁ NOM.mk 3 ⋁ NOM.mk 4).dbl_list_noms
-
---  theorem dream {φ : Form} (h1 : (h₁ :: t₁) = φ.double_list_noms) (h2 : (h₂ :: t₂) = φ.list_noms)
+  theorem all_noc_conj (h : all_nocc i Γ) (L : List Γ) : nom_occurs i (conjunction Γ L) = false := by
+    induction L with
+    | nil => simp [conjunction, nom_occurs]
+    | cons head tail ih =>
+        simp [conjunction, nom_occurs, ih, -Form.conj]
+        exact h head head.2
 
   def Form.bulk_subst : Form → List NOM → List NOM → Form
   | φ, h₁ :: t₁, h₂ :: t₂ => bulk_subst (φ[h₁ // h₂]) t₁ t₂
   | φ, _, []    =>  φ
   | φ, [], _    =>  φ
 
-  def Form.dbl : Form → Form := λ φ => φ.bulk_subst φ.dbl_list_noms φ.list_noms
+  def Form.list_noms : Form → List NOM
+  | nom  i   => [i]
+  | impl φ ψ => (List.merge GE.ge φ.list_noms ψ.list_noms).dedup
+  | box φ    => φ.list_noms
+  | bind _ φ => φ.list_noms
+  | _        => []
 
-  #eval (NOM.mk 2 ⟶ NOM.mk 3 ⟶ NOM.mk 4).dbl
+  def Form.odd_list_noms : Form → List NOM := λ φ => φ.list_noms.map (λ i => 2*i+1)
 
-  lemma new_nom_gt      : nom_occurs i φ → i.letter < φ.new_nom.letter   := by
+  def Form.odd_noms : Form → Form := λ φ => φ.bulk_subst φ.odd_list_noms φ.list_noms
+
+  def Set.odd_noms : Set Form → Set Form := λ Γ => {Form.odd_noms φ | φ ∈ Γ} 
+
+  def nocc_bulk_property (l1 l2 : List NOM) (φ : Form) := ∀ {n : Fin l1.length} {i : NOM}, (i = l1[n]) → (i ∉ φ.list_noms ∨ i ∈ l2.take n) ∧ i ∉ l1.take n
+
+  theorem list_noms_sorted_ge {φ : Form} : φ.list_noms.Sorted GE.ge := by
     induction φ with
-    | nom i          =>
-        simp [nom_occurs, Form.new_nom, -implication_disjunction]
-        intro h
-        rw [h]
-        exact Nat.lt_succ_self i.letter
-    | impl ψ χ ih1 ih2 =>
-        simp only [nom_occurs, Form.new_nom, Bool.or_eq_true, max]
-        intro h
-        apply Or.elim h
-        . intro ha
-          clear ih2 h
-          have ih1 := ih1 ha
-          by_cases hc : (Form.new_nom ψ).letter > (Form.new_nom χ).letter
-          . simp [hc]
-            assumption
-          . simp [hc]
-            simp at hc 
-            exact Nat.lt_of_lt_of_le ih1 hc
-        . intro hb
-          clear ih1 h
-          have ih2 := ih2 hb
-          by_cases hc : (Form.new_nom ψ).letter > (Form.new_nom χ).letter
-          . simp [hc]
-            simp at hc
-            exact Nat.lt_trans ih2 hc
-          . simp [hc]
-            assumption
-    | box      =>
-        assumption
-    | bind     =>
-        assumption
-    | _ => simp [nom_occurs]
-
-  lemma new_nom_is_nom  : nom_occurs (φ.new_nom) φ = false := by
-    rw [←Bool.eq_false_eq_not_eq_true]
-    intro h
-    have a := new_nom_gt h
-    have b := Nat.lt_irrefl φ.new_nom.letter
-    exact b a
+    | nom  i   => simp [Form.list_noms]
+    | impl φ ψ ih1 ih2 =>
+        exact List.Pairwise.sublist ((List.merge GE.ge φ.list_noms ψ.list_noms).dedup_sublist) (List.Sorted.merge ih1 ih2)
+    | box _ ih    => exact ih
+    | bind _ _ ih => exact ih
+    | _        => simp [Form.list_noms]
   
-  lemma ge_new_nom_is_new (h : x ≥ φ.new_nom) : nom_occurs x φ = false := by
-    rw [←Bool.eq_false_eq_not_eq_true]
-    intro habs
-    have := new_nom_gt habs
-    have a := Nat.lt_of_le_of_lt h this
-    have b := Nat.lt_irrefl φ.new_nom.letter
-    exact b a
+  theorem list_noms_nodup {φ : Form} : φ.list_noms.Nodup := by
+    induction φ <;> simp [Form.list_noms, List.nodup_dedup, *]
 
-/-
-  theorem all_lt_list_noms {φ : Form} : ∀ n, n < φ.new_nom.letter → ⟨n⟩ ∈ φ.list_noms := by
-    rw [Form.list_noms]
-    induction φ.new_nom.letter with
-    | zero => simp
-    | succ n ih =>
-        intro i i_lt
-        simp [Form.list_noms.loop] at ih ⊢
-        apply Or.elim (ih i)
-        . intro n_le
-          apply Or.inl
-          apply Nat.le_antisymm
-          apply Nat.lt_add_one_iff.mp
-          assumption
-          assumption
-        . clear i_lt ih
-          intro hmem
-          apply Or.inr
-          assumption
+  theorem list_noms_sorted_gt {φ : Form} : φ.list_noms.Sorted GT.gt := by
+    simp [List.Sorted, List.Pairwise, GT.gt, NOM.gt_iff_ge_and_ne]
+    apply List.Pairwise.and
+    apply list_noms_nodup
+    apply list_noms_sorted_ge
 
-  theorem all_lt_list_noms' {φ : Form} : ∀ n, ⟨n⟩ ∈ φ.list_noms ↔ n < φ.new_nom.letter := by
-    intro n
-    apply Iff.intro
-    . rw [Form.list_noms]
-      induction φ.new_nom.letter with
-      | zero    => simp only [Form.list_noms.loop]; intro; contradiction
-      | succ m ih =>
-          simp [Form.list_noms.loop, -implication_disjunction]
-          intro disj
-          apply Or.elim disj
-          . intro
-            simp [*]
-          . intro
-            simp [*, Nat.lt_succ_of_lt] at *
-    . exact all_lt_list_noms n
--/
+  theorem list_noms_chain' {φ : Form} : φ.list_noms.Chain' GT.gt := by
+    rw [List.chain'_iff_pairwise]
+    exact list_noms_sorted_gt
 
-  -- bit ugly but it works
-  theorem occurs_list_noms : nom_occurs i φ ↔ i ∈ φ.list_noms := by
-    rw [Form.list_noms]
-    apply Iff.intro
-    . intro h
-      have := new_nom_gt h
-      revert this
-      induction φ.new_nom.letter with
-      | zero => simp
-      | succ n ih =>
-          intro h2
-          rw [Form.list_noms.loop]
-          split
-          . simp
-            by_cases heq : i.letter = n
-            . apply Or.inl
-              rw [NOM.mk.injEq]
-              assumption
-            . simp [Nat.lt_succ_iff_lt_or_eq, heq] at h2
-              apply Or.inr; apply ih; assumption
-          . apply ih
-            have : ¬i.letter = n := by
-                intro habs
-                have : i = {letter := n} := by rw [NOM.mk.injEq, habs]
-                simp [*] at *
-            simp [Nat.lt_succ_iff_lt_or_eq, this] at h2
-            assumption
-    . induction φ.new_nom.letter with
-      | zero => simp [Form.list_noms.loop]
-      | succ n ih =>
-          intro h
-          simp [Form.list_noms.loop] at h
-          split at h
-          . simp at h
-            apply Or.elim h
-            . intro; simp [*]
-            . exact ih
-          . apply ih; assumption
-
-  theorem list_noms_subst {old new : NOM} : i ∈ (φ[new // old]).list_noms → ((i ∈ φ.list_noms ∧ i ≠ old) ∨ i = new) := by
-    --rw [all_lt_list_noms', all_lt_list_noms']
-    rw [←occurs_list_noms, ←occurs_list_noms]
-    intro h
-    induction φ with
-    | nom j =>
-        simp [nom_subst_nom] at h
-        split at h
-        . simp [nom_occurs] at h; apply Or.inr; assumption
-        . apply Or.inl
-          apply And.intro
-          . assumption
-          . simp [nom_occurs] at h
-            rw [h]
-            assumption
-    | impl ψ χ ih1 ih2 =>
-        simp [nom_occurs] at h ⊢
-        apply Or.elim h
-        . intro hyp
-          apply Or.elim (ih1 hyp)
-          . intro hl
-            simp [hl]
-          . intro hr
-            simp [hr]
-        . intro hyp
-          apply Or.elim (ih2 hyp)
-          . intro hl
-            simp [hl]
-          . intro hr
-            simp [hr]
-    | box ψ ih =>
-        simp [nom_occurs] at h
-        exact ih h
-    | bind _ ψ ih =>
-        simp [nom_occurs] at h
-        exact ih h
-    | _     => simp [nom_occurs] at h
-
-  theorem occ_bulk {l_new l_old : List NOM} {φ : Form} (eq_len : l_new.length = l_old.length) : nom_occurs i (φ.bulk_subst l_new l_old) → ((i ∈ φ.list_noms ∧ i ∉ l_old) ∨ i ∈ l_new) := by
-    intro h
-    induction l_new generalizing φ l_old with
-    | nil => cases l_old <;> simp [Form.bulk_subst] at *; repeat exact occurs_list_noms.mp h
-    | cons h_new t_new ih =>
-        cases l_old with
-        | nil =>
-            simp [Form.bulk_subst] at h ⊢
-            apply Or.inl
-            exact occurs_list_noms.mp h
-        | cons h_old t_old =>
-            simp [Form.bulk_subst] at eq_len h ⊢
-            have := ih eq_len h
-            apply Or.elim this
-            . intro hyp
-              clear this ih
-              cases t_new
-              . have := List.length_eq_zero.mp (Eq.symm (Eq.subst eq_len (@List.length_nil NOM)))
-                simp [this, Form.bulk_subst] at h ⊢
-                apply Or.elim (list_noms_subst (occurs_list_noms.mp h))
-                . intro c1
-                  simp [c1]
-                . intro c2
-                  exact Or.inr c2
-              . cases t_old
-                . simp at eq_len
-                . simp [Form.bulk_subst] at hyp ⊢
-                  have ⟨a, b⟩ := hyp
-                  apply Or.elim (list_noms_subst b)
-                  . intro c1
-                    apply Or.inl
-                    simp [c1, a]
-                  . intro c2
-                    simp [c2]
-            . intro hyp
-              clear this ih
-              apply Or.inr
-              apply Or.inr
-              assumption
-
-  -- FORM.DBL_LIST_NOMS DOESN'T HAVE THIS PROPERTY
-  theorem nocc_bulk {l_new l_old : List NOM} {φ : Form} (eq_len : l_new.length = l_old.length) : ((i ∉ φ.list_noms ∨ i ∈ l_old) ∧ i ∉ l_new) → nom_occurs i (φ.bulk_subst l_new l_old) = false := by
-    rw [contraposition]
-    simp [-implication_disjunction]
-    intro h1 h2
-    apply Or.elim (occ_bulk eq_len h1)
-    . simp
-    . simp [h2]
-
-  def map_odd : ℕ → NOM → NOM := λ off => λ h => ⟨h.letter*2 + off + (1 - off % 2)⟩ 
-  def map_odd_inv : ℕ → NOM → NOM := λ off => λ h => ⟨(h.letter - (1 - off % 2) - off)/2⟩
-
-  theorem map_odd_inv_is_inv : map_odd_inv off (map_odd off i) = i := by
-    simp [map_odd_inv, map_odd]
-
-  theorem map_odd_ge  : map_odd off i ≥ ⟨off⟩ := by
-    simp [map_odd, NOM.le, Nat.add_comm, Nat.add_assoc]
-
-  def Form.mapping1 : Form → Form := λ φ => φ.bulk_subst (φ.list_noms.map (map_odd φ.new_nom.letter)) φ.list_noms
-  def Form.mapping2 : Form → Form := λ φ =>
-    φ.mapping1.bulk_subst (φ.mapping1.list_noms.map (map_odd_inv φ.new_nom.letter)) φ.mapping1.list_noms
-
-  theorem mapping_inv {φ : Form} : φ.mapping1.mapping2 = φ := by
-    unfold Form.mapping1 Form.mapping2
-    admit 
-
-  theorem mapping1nocc : ∀ i : NOM, i ∈ (φ.list_noms.map (map_odd φ.new_nom.letter)) → nom_occurs i φ = false := by
-    intro i hmem
-    apply ge_new_nom_is_new
-    simp at hmem
-    have ⟨a, p1, _⟩ := hmem
-    have := @map_odd_ge φ.new_nom.letter a
-    rw [p1] at this
-    exact this
-
-  def all_nocc : List NOM → Form → Prop := λ l => λ φ =>  ∀ i, i ∈ l → nom_occurs i φ = false
-
-/-
-  theorem nom_nom_nom_subst {i j a : NOM} (h : nom_occurs i φ = false ∧ nom_occurs j φ = false) : φ[j // a] = φ[i // a][j // i] := by
-    induction φ <;> simp [nom_subst_nom, nom_occurs, *, -implication_disjunction] at *
-    . split <;> simp [nom_subst_nom, Ne.symm, h]
-    . simp [h] at *
-      apply And.intro
-      repeat assumption
-    repeat { simp [h.left, h.right] at *; assumption  }
-
-  -- ((φ[a // b]).bulk_subst l1 l2)
-
-  theorem remember {φ : Form} {h_new : NOM} : (φ.bulk_subst (h_old :: t) t_orig)[h_new // h_old] = φ.bulk_subst (h_new :: t) t_orig := sorry
-
-  theorem triangle_subst {φ : Form} (l₁ l₂ : List NOM) (h1: all_nocc l₁ φ ∧ all_nocc l₂ φ) (h2 : l₁ ≠ [] ∧ l₂ ≠ []) :
-      φ.bulk_subst l₁ φ.list_noms = (φ.bulk_subst l₂ φ.list_noms).bulk_subst l₁ l₂ := by
-      induction φ.list_noms generalizing φ l₁ l₂ with
-      | nil => simp [Form.bulk_subst]; admit
-      | cons h_orig t_orig ih =>
-          cases l₁ with
-          | nil => simp at h2
-          | cons head₁ tail₁ =>
-              cases l₂ with
-              | nil => simp at h2
-              | cons head₂ tail₂ =>
-                  rw [Form.bulk_subst, Form.bulk_subst, remember, Form.bulk_subst]
-                  have nih := @ih (φ[head₁ // h_orig])
-                  clear ih
-
-                  --conv at ih => rhs; rw [Form.bulk_subst, remember]
-                  
-                  --simp only [Form.bulk_subst] at ih ⊢
-                  admit
-      /-
-      cases l₁ with
-      | nil => simp at h5
-      | cons h₁ t₁ =>
-          cases l₂ with
-          | nil => simp at h5
-          | cons h₂ t₂ =>
-              simp [all_nocc, -implication_disjunction] at h1 h2
-              clear h5
-              revert h3 h4
-              cases φ.list_noms
-              . simp [Form.bulk_subst, -implication_disjunction]
-                intro h3 h4
-                rw [h3, h4]
-                admit
-              . simp [Form.bulk_subst, -implication_disjunction]
-                intro h3 h4
-                rw [h4]
-                admit
-        -/
--/
-/-
-  def Form.map_odd_list : Form → List NOM → ℕ → Form 
-  | φ, [], _            => φ
-  | φ, h :: t, offset   => 
-      φ[map_odd_n offset h // h].map_odd_list t offset
-
-  def Form.map_odd      : Form → Form := λ φ => φ.map_odd_list φ.nominals φ.new_nom.letter
-
-  theorem eddie (φ : Form) : φ.map_odd.nominals = φ.nominals.map (map_odd_n φ.new_nom.letter) := by
-    induction φ with
-    | impl ψ χ ih1 ih2 =>
-        simp [Form.map_odd]        
-        admit
-    | _ => admit 
-
-  theorem helper {φ : Form} : ∀ i : NOM, nom_occurs i φ.map_odd → i ≥ φ.new_nom := by
-    intro i
-    rw [Form.map_odd]
-    have h : φ.nominals = [] ↔ ∀ i : NOM, nom_occurs i φ = false := hmm φ
-    revert h
-    induction φ.nominals generalizing φ with
-    | nil =>
-        simp only [true_iff, Form.map_odd_list, ge_iff_le]
-        intro a b
-        exfalso
-        have := Eq.mpr (Bool.eq_false_eq_not_eq_true (nom_occurs i φ)) (a i)
-        contradiction
-    | cons h t ih =>
-        let ψ : Form := sorry
-        have : t = ψ.nominals := sorry
-        rw [this] at ih
-        have new_ih := ih (hmm ψ)
-        clear ih
-        simp only [Form.map_odd_list]
-        intro c hocc
-        clear c
-        admit
-
-  def Form.double_list : Form → List NOM → Form
-  | φ, []       => φ
-  | φ, h :: t   => φ [NOM.mk (h.letter * 2) // h].double_list t
-
-  def Form.half_list : Form → List NOM → Form
-  | φ, []       => φ
-  | φ, h :: t   => φ [NOM.mk (h.letter / 2) // h].double_list t
-
-  def Form.double  : Form → Form   :=   λ φ => φ.double_list (φ.nominals)
-  def Form.half    : Form → Form   :=   λ φ => φ.half_list (φ.nominals)
-
---  notation:150 φ "*2" => Form.double φ
---  notation:150 φ "/2" => Form.half φ
-
-  def Set.double : Set Form → Set Form := λ Γ => {Form.double φ | φ ∈ Γ}
-  def Set.half   : Set Form → Set Form := λ Γ => {Form.half φ | φ ∈ Γ}
-
-  def Form.double_n : Form → ℕ → Form
-  | φ, 0         => φ
-  | φ, n+1       => (nom_subst_nom φ ⟨2*(n+1)⟩ ⟨n+1⟩).double_n n
-
-  def Form.double'  : Form → Form   := λ φ => φ.double_n φ.new_nom.letter
-
-  def Form.double''  : Form → Form   := λ φ =>
-    loop φ φ.new_nom.letter
-  where
-    loop : Form → ℕ → Form
-    | φ, 0      => φ
-    | φ, n+1    => loop (nom_subst_nom φ ⟨2*n⟩ ⟨n⟩) n
-
-
-  #eval (NOM.mk 3 ⋁ NOM.mk 6).double''
---  notation:150 Γ "*2" => Set.double Γ 
---  notation:150 Γ "/2" => Set.half Γ 
--/
 end NominalSubstitution
 
 section IteratedModalities
@@ -899,3 +355,9 @@ section IteratedModalities
 
 
 end IteratedModalities
+
+  theorem ex_depth {x : SVAR} : Form.depth φ < Form.depth (ex x, φ) := by
+    simp [Form.depth]
+    rw [←Nat.add_assoc, ←Nat.add_assoc, Nat.add_comm]
+    apply Nat.lt_add_of_pos_right
+    simp
