Hybrid/Lindenbaum.lean
@@ -1,237 +1,333 @@
+import Hybrid.Substitutions
 import Hybrid.ProofUtils
 import Hybrid.FormCountable
 
 open Classical
 
-section Lindenbaum
+-- First, we define how to obtain Γᵢ₊₁ from Γᵢ, given a formula φ: 
+def lindenbaum_next (Γ : Set Form) (φ : Form) : Set Form :=
+  if (Γ ∪ {φ}).consistent then
+    match φ with
+    | ex x, ψ =>
+        if c : ∃ i : NOM, all_nocc i (Γ ∪ {φ}) then
+          Γ ∪ {φ} ∪ {ψ[c.choose // x]}
+        else
+          Γ ∪ {φ}
+    | _       =>  Γ ∪ {φ}
+  else
+    Γ
 
-  -- First, we define how to obtain Γᵢ₊₁ from Γᵢ, given a formula φ: 
-  def lindenbaum_next (Γ : Set Form) (φ : Form) : Set Form :=
-    if (Γ ∪ {φ}).consistent then
-      Γ ∪ {φ}
-    else
-      Γ
-  
-  -- Now we define the whole indexed family Γᵢ.
-  -- Usually, the enumeration of formulas starts from 1 (φ₁, φ₂, ...), and
-  --    Γ₀ = Γ .
-  -- However, in Lean it's much tidier to enumerate from 0 (φ₀, φ₁, ...), so
-  --    Γ₀ = Γ ∪ {φ₀} if it is consistent and Γ₀ = Γ otherwise.
-  def lindenbaum_family (enum : Nat → Form) (Γ : Set Form) : Nat → Set Form 
-  | .zero   => lindenbaum_next Γ (enum 0)
-  | .succ n =>
-      let prev_set := lindenbaum_family enum Γ n
-      lindenbaum_next prev_set (enum (n+1))
-  
-  notation Γ "(" i "," e ")" => lindenbaum_family e Γ i    
+-- Now we define the whole indexed family Γᵢ.
+-- Usually, the enumeration of formulas starts from 1 (φ₁, φ₂, ...), and
+--    Γ₀ = Γ .
+-- However, in Lean it's much tidier to enumerate from 0 (φ₀, φ₁, ...), so
+--    Γ₀ = Γ ∪ {φ₀} if it is consistent and Γ₀ = Γ otherwise.
+def lindenbaum_family (enum : Nat → Form) (Γ : Set Form) : Nat → Set Form 
+| .zero   => lindenbaum_next Γ (enum 0)
+| .succ n =>
+    let prev_set := lindenbaum_family enum Γ n
+    lindenbaum_next prev_set (enum (n+1))
 
-  def LindenbaumMCS (enum : Nat → Form) (Γ : Set Form) (_ : Γ.consistent) : Set Form :=
-      {φ | ∃ i : Nat, φ ∈ Γ (i, enum)}
+notation Γ "(" i "," e ")" => lindenbaum_family e Γ i    
 
-  -- Lemma: All Γᵢ belong to LindenbaumMCS Γ
-  lemma all_sets_in_family{enum : ℕ → Form} {Γ : Set Form} {c : Γ.consistent} : ∀ n, Γ (n, enum) ⊆ LindenbaumMCS enum Γ c := by
-    intro i φ h
-    exists i
-  
-  lemma all_sets_in_family_tollens {enum : ℕ → Form} {Γ : Set Form} {c : Γ.consistent} : φ ∉ (LindenbaumMCS enum Γ c) → ∀ n, φ ∉ Γ (n, enum) := by
-    rw [contraposition, not_not, not_forall]
-    intro h
-    let ⟨i, hi⟩ := h
-    rw [not_not] at hi
-    exact all_sets_in_family i hi 
+def LindenbaumMCS (enum : Nat → Form) (Γ : Set Form) (_ : Γ.consistent) : Set Form :=
+    {φ | ∃ i : Nat, φ ∈ Γ (i, enum)}
 
-  -- Lemma: If Γ is consistent, then for all φ, lindenbaum_next Γ φ is consistent
-  lemma consistent_lindenbaum_next (Γ : Set Form) (hc : Γ.consistent) (φ : Form) : (lindenbaum_next Γ φ).consistent := by
-    rw [lindenbaum_next]
-    split <;> assumption
-  
-  -- Lemma: If you can consistently extend (lindenbaum_next Γ φ) with φ, then
-  --    φ already belongs to (lindenbaum_next Γ φ)
-  lemma maximal_lindenbaum_next {Γ : Set Form} (hc : ((lindenbaum_next Γ φ) ∪ {φ}).consistent) : φ ∈ lindenbaum_next Γ φ := by
-    rw [lindenbaum_next] at hc
-    by_cases h : (Γ ∪ {φ}).consistent
-    . clear hc
-      simp only [lindenbaum_next, h, ite_true]
-      simp only [Set.union_singleton, Set.mem_insert_iff, true_or]
-    . simp only [h, ite_false] at hc
-      -- ^ contradiction
+-- Lemma: All Γᵢ belong to LindenbaumMCS Γ
+lemma all_sets_in_family{enum : ℕ → Form} {Γ : Set Form} {c : Γ.consistent} : ∀ n, Γ (n, enum) ⊆ LindenbaumMCS enum Γ c := by
+  intro i φ h
+  exists i
 
-  --
-  -- Now apply the previous lemmas to the family as a whole.
-  --
+lemma all_sets_in_family_tollens {enum : ℕ → Form} {Γ : Set Form} {c : Γ.consistent} : φ ∉ (LindenbaumMCS enum Γ c) → ∀ n, φ ∉ Γ (n, enum) := by
+  rw [contraposition, not_not, not_forall]
+  intro h
+  let ⟨i, hi⟩ := h
+  rw [not_not] at hi
+  exact all_sets_in_family i hi 
 
-  -- Lemma: If Γ is consistent, then all Γᵢ are consistent.
-  lemma consistent_family {Γ : Set Form} (e : ℕ → Form) (c : Γ.consistent) : ∀ n, (Γ (n, e)).consistent := by
-    intro n
-    induction n with
-    | zero =>
-        simp only [lindenbaum_family, lindenbaum_next]
-        split <;> assumption
-    | succ n ih =>
-        simp only [lindenbaum_family]
-        apply consistent_lindenbaum_next
-        assumption
+-- Lemma: If Γ is consistent, then for all φ, lindenbaum_next Γ φ is consistent
+lemma consistent_lindenbaum_next (Γ : Set Form) (hc : Γ.consistent) (φ : Form) : (lindenbaum_next Γ φ).consistent := by
+  rw [lindenbaum_next]
+  split
+  . split
+    . next x ψ h =>
+      split
+      . next hnom =>
+        let i := Exists.choose hnom
+        have not1 : i = Exists.choose hnom := by simp
+        have i_sat := Exists.choose_spec hnom
+        have not2 : (ex x, ψ) = ((all x, ψ⟶⊥)⟶⊥) := by simp
+        rw [←not1, ←not2, Set.consistent, ←Proof.Deduction, SyntacticConsequence]
+        intro ⟨L, habs⟩
+        let χ := conjunction (Γ ∪ {ex x, ψ}) L
+        have not3 : χ = conjunction (Γ ∪ {ex x, ψ}) L := by simp
+        rw [←not3] at habs
+        let y := (χ⟶ψ).new_var
+        have y_ge : y ≥ (χ⟶ψ).new_var := by simp [SVAR.le]
+        have : y ≥ (χ⟶(ψ[i//x])⟶⊥).new_var := ge_new_var_subst_helpr y_ge
+        have habs := (Proof.generalize_constants i this) habs
+        rw [nom_subst_svar, nom_subst_svar] at habs
+        have nocc0 : occurs y χ = false := by apply ge_new_var_is_new; exact (new_var_geq1 y_ge).left
+        have nocc1 : nom_occurs i χ = false := all_noc_conj i_sat L
+        conv at i_sat =>
+          rw [←not1, ←not2, all_nocc, Set.union_singleton]
+          intro φ; rw [Set.mem_insert_iff]
+        have nocc2 : nom_occurs i (ex x, ψ) = false := by apply (i_sat (ex x, ψ)); simp
+        simp only [nom_occurs, or_false, Bool.or_false, ←not1] at nocc2
+        rw [nom_subst_nocc nocc1, subst_collect_all_nocc nocc2] at habs
+        have := Proof.ax_q1 χ (ψ[y//x]⟶⊥) (notoccurs_notfree nocc0)
+        have habs := Proof.mp this habs
+        have habs : ∃ L, ⊢(conjunction (Γ ∪ {ex x, ψ}) L⟶all y, ψ[y//x]⟶⊥) := ⟨L, habs⟩
+        rw [←SyntacticConsequence, ←Form.neg] at habs
+        have : ⊢((all y, ∼(ψ[y//x])) ⟶ (all x, ∼ψ)) := by
+          apply Proof.iff_mpr
+          apply Proof.rename_bound
+          apply ge_new_var_is_new
+          rw [new_var_neg]
+          exact (new_var_geq1 y_ge).right
+          rw [subst_neg]
+          apply new_var_subst'' (new_var_geq1 y_ge).right
+        have := Proof.Γ_theorem this (Γ ∪ {ex x, ψ})
+        have habs := Proof.Γ_mp this habs 
+        have : (Γ ∪ {ex x, ψ}) ⊢ (ex x, ψ) := by apply Proof.Γ_premise; simp
+        have := Proof.Γ_mp this habs
+        contradiction
+      . assumption
+    . assumption
+  . assumption
 
-  -- Lemma: If φ doesn't belong to the set in the family corresponding to its place in the enumeration,
-  --     (i.e., φ ∉ Γᵢ, where i = f φ),
-  --    then Γᵢ ∪ {φ} must be inconsistent.
-  lemma maximal_family {Γ : Set Form} {f : Form → ℕ} (f_inj : f.Injective) {e : ℕ → Form} (e_inv : e = f.invFun) :
-      ¬φ ∈ Γ (f φ, e) → ¬(Γ (f φ, e) ∪ {φ}).consistent := by
-      rw [contraposition, not_not, not_not]
-      unfold lindenbaum_family
-      cases heq : f φ with
-      | zero =>
-          simp only
-          have by_inv : e (f φ) = φ := by simp [f.leftInverse_invFun f_inj φ, e_inv]
-          rw [show 0 = f φ by simp [heq], by_inv]
-          intro h
-          rw [lindenbaum_next]
-          apply maximal_lindenbaum_next
-          exact h
-      | succ n =>
-          simp only
-          have by_inv : e (f φ) = φ := by simp [f.leftInverse_invFun f_inj φ, e_inv]
-          simp only [show (n+1) = f φ by simp [heq], by_inv]
-          intro h
-          rw [lindenbaum_next]
-          apply maximal_lindenbaum_next
-          exact h
 
-  -- todo: Include here that Γ ⊆ Γᵢ for all i
-  lemma increasing_family : i ≤ j → Γ (i, e) ⊆ Γ (j, e) := by
-    intro h
-    induction h with
-    | refl => simp [subset_of_eq]
-    | @step m _ ih =>
-        simp only [lindenbaum_family, lindenbaum_next]
-        split
-        . intro _ φ_member
-          have incl : Γ(m, e) ⊆ (Γ(m, e) ∪ {e (m + 1)}) := by simp
-          exact incl (ih φ_member)
-        . assumption
-  
-  -- Now we want to show that Γ' = LindenbaumMCS e Γ is consistent.
-  --
-  -- (f is an injection Form → ℕ  ; e is its (left) inverse ℕ → Form)
-  --
-  -- Assume Γ' is inconsistent.
-  --  That means that there is list of elements L of that set
-  --  such that their conjunction proves a contradiction.
-  --
-  -- L : List (LindenbaumMCS e Γ)
-  --   there is a "maximum formula" in L, (Prove!)
-  --   i.e. a formula φ s.t. for all ψ ≠ φ in L f(φ) > f(ψ)
-  -- Clearly, φ ∈ lindenbaum_family e Γ f(φ). (lemma in_set)
-  -- Now, we know that for all formulas ψ, if f(ψ) <= n, then
-  --    ψ ∈ lindenbaum_family e Γ n. (Prove!)
-  -- So since φ is the greatest element in L, then all elements in L
-  --    are elements in lindenbaum_family e Γ f(φ).
-  -- So in fact L only contains elements from lindenbaum_family e Γ f(φ),
-  --    not from the whole MCS.
-  --
-  -- We know that if Γ is consistent, then for all n, lindenbaum_family e Γ n
-  --    is consistent. (lemma consistent_family).
-  -- So lindenbaum_family e Γ f(φ) is consistent.
-  -- So no conjunction of elements in L can prove a contradiction.
-  --
-  --    This completes our reductio proof.
-  --    We conclude LindenbaumMCS e Γ is consistent after all.
+-- Lemma: If you can consistently extend (lindenbaum_next Γ φ) with φ, then
+--    φ already belongs to (lindenbaum_next Γ φ)
+lemma maximal_lindenbaum_next {Γ : Set Form} (hc : ((lindenbaum_next Γ φ) ∪ {φ}).consistent) : φ ∈ lindenbaum_next Γ φ := by
+  revert hc
+  rw [lindenbaum_next]
+  split
+  . split
+    . split <;> simp
+    . intro; simp
+  . intro; contradiction
 
-  -- Needed, but unrelated.
-  lemma incl_insert {A B : Set α} (h1 : A ⊆ B) (h2 : x ∈ B) : (A ∪ {x}) ⊆ B := by
-    intro a h
-    simp at h
-    apply Or.elim h
-    . intro ax
-      rw [ax]
+--
+-- Now apply the previous lemmas to the family as a whole.
+--
+
+-- Lemma: If Γ is consistent, then all Γᵢ are consistent.
+lemma consistent_family {Γ : Set Form} (e : ℕ → Form) (c : Γ.consistent) : ∀ n, (Γ (n, e)).consistent := by
+  intro n
+  induction n <;> (
+      simp only [lindenbaum_family]
+      apply consistent_lindenbaum_next
       assumption
-    . apply h1
-  
-  -- If φ is a formula that belongs to the infinite union Γ' = LindenbaumMCS e Γ,
-  --    then φ must belong to some Γᵢ from Γ'.
-  -- More specifically, i = f φ; i.e. the place of φ in the enumeration.
-  lemma at_finite_step {Γ : Set Form} (c : Γ.consistent) (f : Form → ℕ) (f_inj : f.Injective) (e : ℕ → Form) (e_inv : e = f.invFun) :
-      φ ∈ LindenbaumMCS e Γ c → φ ∈ Γ (f φ, e) := by
-    rw [contraposition]
-    simp only [LindenbaumMCS, Set.mem_setOf_eq, not_exists, not_not]
-    intro h n habs
-    by_cases order : n ≤ (f φ)
-    . have incl := increasing_family order habs
-      contradiction
-    . simp only [not_le] at order
-      have order := Nat.le_of_lt order
-      have incl := incl_insert (@increasing_family (f φ) n e Γ order) habs
-      have n_consistent := consistent_family e c n
-      have phi_inconsistent := maximal_family f_inj e_inv h
-      clear h
-      simp only [Set.consistent, not_not] at n_consistent phi_inconsistent
-      have n_inconsistent := Proof.increasing_consequence phi_inconsistent incl
-      exact n_consistent n_inconsistent
+  )
 
-  -- Given a finite list of elements in (LindenbaumMCS e Γ c), all elements of that list
-  --    occur in some Γᵢ that makes up the infinite union.
-  lemma list_at_finite_step {Γ : Set Form} {c : Γ.consistent} (f : Form → ℕ) (f_inj : f.Injective) (e : ℕ → Form) (e_inv : e = f.invFun) (L : List (LindenbaumMCS e Γ c)) :
-      {↑φ | φ ∈ L} ⊆ (Γ (L.max_form f, e)) := by
-      intro φ_val hmem
-      simp only [Set.mem_setOf_eq] at hmem
-      let ⟨φ, φ_property, φ_is_val⟩ := hmem
-      rw [←φ_is_val]
-      clear hmem φ_val φ_is_val
-      have φ_in_MCS : ↑φ ∈ LindenbaumMCS e Γ c := by simp
-      have φ_in_own_set := at_finite_step c f f_inj e e_inv φ_in_MCS
-      have := L.max_is_max f φ φ_property
-      exact increasing_family this φ_in_own_set
+-- Lemma: If φ doesn't belong to the set in the family corresponding to its place in the enumeration,
+--     (i.e., φ ∉ Γᵢ, where i = f φ),
+--    then Γᵢ ∪ {φ} must be inconsistent.
+lemma maximal_family {Γ : Set Form} {f : Form → ℕ} (f_inj : f.Injective) {e : ℕ → Form} (e_inv : e = f.invFun) :
+    ¬φ ∈ Γ (f φ, e) → ¬(Γ (f φ, e) ∪ {φ}).consistent := by
+    rw [contraposition, not_not, not_not]
+    unfold lindenbaum_family
+    cases heq : f φ with
+    | zero =>
+        simp only
+        have by_inv : e (f φ) = φ := by simp [f.leftInverse_invFun f_inj φ, e_inv]
+        rw [show 0 = f φ by simp [heq], by_inv]
+        intro h
+        rw [lindenbaum_next]
+        apply maximal_lindenbaum_next
+        exact h
+    | succ n =>
+        simp only
+        have by_inv : e (f φ) = φ := by simp [f.leftInverse_invFun f_inj φ, e_inv]
+        simp only [show (n+1) = f φ by simp [heq], by_inv]
+        intro h
+        rw [lindenbaum_next]
+        apply maximal_lindenbaum_next
+        exact h
 
-  lemma LindenbaumConsistent {Γ : Set Form} (c : Γ.consistent) {f : Form → ℕ} (f_inj : f.Injective) {e : ℕ → Form} (e_inv : e = f.invFun) :
-    (LindenbaumMCS e Γ c).consistent := by
-    rw [←@not_not (Set.consistent (LindenbaumMCS e Γ c))]
-    intro habs
-    rw [Set.consistent, not_not, SyntacticConsequence] at habs
-    let ⟨L, L_incons⟩ := habs
-    clear habs
-    let ⟨L', conj_L'⟩ := conj_incl_linden L (list_at_finite_step f f_inj e e_inv L)
-    rw [conj_L'] at L_incons
-    clear conj_L'
-    have : ((⊢(conjunction (Γ(L.max_form f, e)) L'⟶⊥) → (Γ(L.max_form f, e)) ⊢ ⊥)) := by intro h; simp [SyntacticConsequence]; exists L'
-    have := this L_incons
-    have := consistent_family e c (L.max_form f)
+-- todo: Include here that Γ ⊆ Γᵢ for all i
+lemma increasing_family : i ≤ j → Γ (i, e) ⊆ Γ (j, e) := by
+  intro h
+  induction h with
+  | refl => simp [subset_of_eq]
+  | @step m _ ih =>
+      simp only [lindenbaum_family, lindenbaum_next]
+      split
+      . intro _ φ_member
+        have incl : Γ(m, e) ⊆ (Γ(m, e) ∪ {e (m + 1)}) := by simp
+        split ; split
+        . rw [Set.union_singleton]
+          apply Set.subset_insert
+          exact incl (ih φ_member)
+        . exact incl (ih φ_member)
+        . exact incl (ih φ_member)
+      . assumption
+
+lemma Γ_in_family : Γ ⊆ Γ (i, e) := by
+  induction i with
+  | zero =>
+      simp only [lindenbaum_family, lindenbaum_next]
+      split ; split ; split
+      . apply subset_trans
+        have : Γ ⊆ Γ ∪ {e 0} := by simp
+        exact this
+        simp
+      . simp
+      . simp
+      . apply subset_of_eq
+        simp
+  | succ n ih =>
+      apply subset_trans
+      apply ih
+      apply increasing_family
+      apply Nat.le_succ
+
+-- Now we want to show that Γ' = LindenbaumMCS e Γ is consistent.
+--
+-- (f is an injection Form → ℕ  ; e is its (left) inverse ℕ → Form)
+--
+-- Assume Γ' is inconsistent.
+--  That means that there is list of elements L of that set
+--  such that their conjunction proves a contradiction.
+--
+-- L : List (LindenbaumMCS e Γ)
+--   there is a "maximum formula" in L, (Prove!)
+--   i.e. a formula φ s.t. for all ψ ≠ φ in L f(φ) > f(ψ)
+-- Clearly, φ ∈ lindenbaum_family e Γ f(φ). (lemma in_set)
+-- Now, we know that for all formulas ψ, if f(ψ) <= n, then
+--    ψ ∈ lindenbaum_family e Γ n. (Prove!)
+-- So since φ is the greatest element in L, then all elements in L
+--    are elements in lindenbaum_family e Γ f(φ).
+-- So in fact L only contains elements from lindenbaum_family e Γ f(φ),
+--    not from the whole MCS.
+--
+-- We know that if Γ is consistent, then for all n, lindenbaum_family e Γ n
+--    is consistent. (lemma consistent_family).
+-- So lindenbaum_family e Γ f(φ) is consistent.
+-- So no conjunction of elements in L can prove a contradiction.
+--
+--    This completes our reductio proof.
+--    We conclude LindenbaumMCS e Γ is consistent after all.
+
+-- Needed, but unrelated.
+lemma incl_insert {A B : Set α} (h1 : A ⊆ B) (h2 : x ∈ B) : (A ∪ {x}) ⊆ B := by
+  intro a h
+  simp at h
+  apply Or.elim h
+  . intro ax
+    rw [ax]
+    assumption
+  . apply h1
+
+-- If φ is a formula that belongs to the infinite union Γ' = LindenbaumMCS e Γ,
+--    then φ must belong to some Γᵢ from Γ'.
+-- More specifically, i = f φ; i.e. the place of φ in the enumeration.
+lemma at_finite_step {Γ : Set Form} (c : Γ.consistent) (f : Form → ℕ) (f_inj : f.Injective) (e : ℕ → Form) (e_inv : e = f.invFun) :
+    φ ∈ LindenbaumMCS e Γ c → φ ∈ Γ (f φ, e) := by
+  rw [contraposition]
+  simp only [LindenbaumMCS, Set.mem_setOf_eq, not_exists, not_not]
+  intro h n habs
+  by_cases order : n ≤ (f φ)
+  . have incl := increasing_family order habs
     contradiction
+  . simp only [not_le] at order
+    have order := Nat.le_of_lt order
+    have incl := incl_insert ((@increasing_family (f φ)) order) habs
+    have n_consistent := consistent_family e c n
+    have phi_inconsistent := maximal_family f_inj e_inv h
+    clear h
+    simp only [Set.consistent, not_not] at n_consistent phi_inconsistent
+    have n_inconsistent := Proof.increasing_consequence phi_inconsistent incl
+    exact n_consistent n_inconsistent
 
-  lemma LindenbaumMaximal {Γ : Set Form} (c : Γ.consistent) {f : Form → ℕ} (f_inj : f.Injective) {e : ℕ → Form} (e_inv : e = f.invFun) :
-    ∀ φ, φ ∉ (LindenbaumMCS e Γ c) → ((LindenbaumMCS e Γ c) ∪ {φ}) ⊢ ⊥ := by
-    intro φ not_mem
-    have := all_sets_in_family_tollens not_mem (f φ)
-    have := maximal_family f_inj e_inv this
-    simp only [Set.consistent, not_not, ←Proof.Deduction] at this ⊢
-    apply Proof.increasing_consequence this
-    apply all_sets_in_family
+-- Given a finite list of elements in (LindenbaumMCS e Γ c), all elements of that list
+--    occur in some Γᵢ that makes up the infinite union.
+lemma list_at_finite_step {Γ : Set Form} {c : Γ.consistent} (f : Form → ℕ) (f_inj : f.Injective) (e : ℕ → Form) (e_inv : e = f.invFun) (L : List (LindenbaumMCS e Γ c)) :
+    {↑φ | φ ∈ L} ⊆ (Γ (L.max_form f, e)) := by
+    intro φ_val hmem
+    simp only [Set.mem_setOf_eq] at hmem
+    let ⟨φ, φ_property, φ_is_val⟩ := hmem
+    rw [←φ_is_val]
+    clear hmem φ_val φ_is_val
+    have φ_in_MCS : ↑φ ∈ LindenbaumMCS e Γ c := by simp
+    have φ_in_own_set := at_finite_step c f f_inj e e_inv φ_in_MCS
+    have := L.max_is_max f φ φ_property
+    exact increasing_family this φ_in_own_set
 
-  theorem LindenbaumLemma : ∀ Γ : Set Form, Γ.consistent → ∃ Γ' : Set Form, Γ ⊆ Γ' ∧ Γ'.MCS := by
-    intro Γ cons
-    let ⟨f, f_inj⟩ := exists_injective_nat Form
-    let enum       := f.invFun
-    let Γ' := LindenbaumMCS enum Γ cons
-    have enum_inv : enum = f.invFun := by simp
-    exists Γ'
-    apply And.intro 
-    . -- Γ is included in Γ'
-      let Γ₀ := Γ (0, enum)
-      have Γ_in_Γ₀ : Γ ⊆ Γ₀ := by
-          simp [show Γ₀ = Γ (0, enum) by simp, lindenbaum_family, lindenbaum_next]
-          split <;> simp [subset_of_eq]
-      have Γ₀_in_family := @all_sets_in_family enum Γ cons 0
-      rw [show LindenbaumMCS enum Γ cons = Γ' by simp, show Γ (0, enum) = Γ₀ by simp] at Γ₀_in_family
-      intro _ φ_in_Γ
-      exact Γ₀_in_family (Γ_in_Γ₀ φ_in_Γ)
-    . rw [Set.MCS]
-      apply And.intro
-      . exact LindenbaumConsistent cons f_inj enum_inv
-      . exact LindenbaumMaximal cons f_inj enum_inv
+lemma LindenbaumConsistent {Γ : Set Form} (c : Γ.consistent) {f : Form → ℕ} (f_inj : f.Injective) {e : ℕ → Form} (e_inv : e = f.invFun) :
+  (LindenbaumMCS e Γ c).consistent := by
+  rw [←@not_not (Set.consistent (LindenbaumMCS e Γ c))]
+  intro habs
+  rw [Set.consistent, not_not, SyntacticConsequence] at habs
+  let ⟨L, L_incons⟩ := habs
+  clear habs
+  let ⟨L', conj_L'⟩ := conj_incl_linden L (list_at_finite_step f f_inj e e_inv L)
+  rw [conj_L'] at L_incons
+  clear conj_L'
+  have : ((⊢(conjunction (Γ(L.max_form f, e)) L'⟶⊥) → (Γ(L.max_form f, e)) ⊢ ⊥)) := by intro h; simp [SyntacticConsequence]; exists L'
+  have := this L_incons
+  have := consistent_family e c (L.max_form f)
+  contradiction
 
-end Lindenbaum
+lemma LindenbaumMaximal {Γ : Set Form} (c : Γ.consistent) {f : Form → ℕ} (f_inj : f.Injective) {e : ℕ → Form} (e_inv : e = f.invFun) :
+  ∀ φ, φ ∉ (LindenbaumMCS e Γ c) → ((LindenbaumMCS e Γ c) ∪ {φ}) ⊢ ⊥ := by
+  intro φ not_mem
+  have := all_sets_in_family_tollens not_mem (f φ)
+  have := maximal_family f_inj e_inv this
+  simp only [Set.consistent, not_not, ←Proof.Deduction] at this ⊢
+  apply Proof.increasing_consequence this
+  apply all_sets_in_family
 
-/-
-theorem ExtendedLindenbaumLemma : ∀ Γ : Set Form, Γ.consistent → ∃ Γ' : Set Form, Γ.double ⊆ Γ' ∧ Γ'.witnessed ∧ Γ'.MCS := by
+theorem RegularLindenbaumLemma : ∀ Γ : Set Form, Γ.consistent → ∃ Γ' : Set Form, Γ ⊆ Γ' ∧ Γ'.MCS := by
   intro Γ cons
-  admit
--/
+  let ⟨f, f_inj⟩ := exists_injective_nat Form
+  let enum       := f.invFun
+  let Γ' := LindenbaumMCS enum Γ cons
+  have enum_inv : enum = f.invFun := rfl
+  exists Γ'
+  apply And.intro 
+  . -- Γ is included in Γ'
+    let Γ₀ := Γ (0, enum)
+    have Γ_in_Γ₀ : Γ ⊆ Γ₀ := Γ_in_family
+    have Γ₀_in_family := @all_sets_in_family enum Γ cons 0
+    rw [show LindenbaumMCS enum Γ cons = Γ' by simp, show Γ (0, enum) = Γ₀ by simp] at Γ₀_in_family
+    intro _ φ_in_Γ
+    exact Γ₀_in_family (Γ_in_Γ₀ φ_in_Γ)
+  . rw [Set.MCS]
+    apply And.intro
+    . exact LindenbaumConsistent cons f_inj enum_inv
+    . intro φ
+      exact LindenbaumMaximal cons f_inj enum_inv φ
+
+def Set.enough_noms (Γ : Set Form) := (∃ i, all_nocc i Γ) ∧ ∀ (e : ℕ → Form) (n : ℕ), ∃ i, all_nocc i (Γ (n, e))
+
+lemma LindenbaumWitnessed {Γ : Set Form} (c : Γ.consistent) {f : Form → ℕ} (f_inj : f.Injective) {e : ℕ → Form} (e_inv : e = f.invFun)
+    (h : Γ.enough_noms) : (LindenbaumMCS e Γ c).witnessed := by
+    intro φ φ_mem
+    split
+    . next φ x ψ =>
+        have φ_mem := at_finite_step c f f_inj e e_inv φ_mem
+        let n := f ((all x, ψ⟶⊥)⟶⊥)
+        have not₁ : n = f ((all x, ψ⟶⊥)⟶⊥) := by simp
+        have not₂ : (ex x, ψ) = ((all x, ψ⟶⊥)⟶⊥) := by simp
+        rw [←not₁, ←not₂] at φ_mem
+
+        have ⟨i, nocc⟩ := h.right e n
+        exists i
+        apply all_sets_in_family (n)
+        revert not₁
+        cases n with
+        | zero =>
+            intro not₁
+            have : e (Nat.zero) = ((all x, ψ⟶⊥)⟶⊥) := by rw [not₁, e_inv, Function.leftInverse_invFun f_inj]
+            rw [lindenbaum_family, this, lindenbaum_next]
+            admit
+        | succ n =>
+            intro not₁
+            simp [lindenbaum_family]
+            admit
+
+    . assumption
+
+theorem ExtendedLindenbaumLemma : ∀ Γ : Set Form, Γ.consistent → ∃ Γ' : Set Form, Γ.odd_noms ⊆ Γ' ∧ Γ'.MCS ∧ Γ'.witnessed := by admit
