Hybrid/Tautology.lean
@@ -28,16 +28,53 @@ syntax "eval" : tactic
 macro_rules
   | `(tactic| eval) => `(tactic| intro e; simp [e.p1, e.p2, e_dn, e_neg, e_conj, e_disj, e_impl, -Form.neg, -Form.conj, -Form.disj, -Form.iff])
 
-theorem hs : Tautology ((φ ⟶ ψ) ⟶ (ψ ⟶ χ) ⟶ (φ ⟶ χ)) := by
+theorem hs_taut : Tautology ((φ ⟶ ψ) ⟶ (ψ ⟶ χ) ⟶ (φ ⟶ χ)) := by
     admit
 
 theorem ax_1 : Tautology (φ ⟶ ψ ⟶ φ) := by
   intro e
   simp only [e.p2, Bool.not_eq_true, or_comm, ←or_assoc, Bool.dichotomy, true_or]
 
+theorem neg_conj : Tautology ((φ ⟶ ∼ψ) ⟷ ∼(φ ⋀ ψ)) := by
+  simp
+  eval
+
+theorem contrapositive : Tautology ((φ ⟶ ψ) ⟶ (∼ψ ⟶ ∼φ)) := by
+  eval
+  simp only [or_comm]
+  simp only [and_or_right]
+  apply And.intro
+  . rw [←or_assoc, ←Bool.not_eq_true]
+    apply Or.inl
+    apply em
+  . rw [←or_comm, or_assoc, or_comm, ←Bool.not_eq_true]
+    apply Or.inl
+    apply em
+
+theorem contrapositive' : Tautology ((∼ψ ⟶ ∼φ) ⟶ (φ ⟶ ψ)) := by
+  eval
+  simp only [or_comm]
+  simp only [and_or_right]
+  apply And.intro
+  . rw [←or_assoc, ←Bool.not_eq_true]
+    apply Or.inl
+    rw [or_comm]
+    apply em
+  . rw [←or_comm, or_assoc, or_comm, ←Bool.not_eq_true]
+    apply Or.inl
+    rw [or_comm]
+    apply em
+
 theorem neg_intro : Tautology ((φ ⟶ ψ) ⟶ (φ ⟶ ∼ψ) ⟶ ∼φ) := by
     eval
     admit
+
+theorem imp_refl : Tautology (φ ⟶ φ) := by
+  eval
+
+theorem imp_neg : Tautology (∼(φ ⟶ ψ) ⟷ (φ ⋀ ∼ψ)) := by
+  simp only [Form.iff, Form.conj, Form.neg]
+  eval
 
 theorem dne : Tautology (∼∼φ ⟶ φ) := by
   eval
@@ -54,6 +91,10 @@ theorem conj_intro : Tautology (φ ⟶ ψ ⟶ (φ ⋀ ψ)) := by
   eval
   admit
 
+theorem conj_intro_hs : Tautology ((φ ⟶ ψ) ⟶ (φ ⟶ χ) ⟶ (φ ⟶ (ψ ⋀ χ))) := by
+  eval
+  admit
+
 theorem conj_elim_l : Tautology ((φ ⋀ ψ) ⟶ φ) := by
   eval
   simp [←or_assoc, or_comm, Bool.dichotomy]
@@ -61,6 +102,42 @@ theorem conj_elim_l : Tautology ((φ ⋀ ψ) ⟶ φ) := by
 theorem conj_elim_r : Tautology ((φ ⋀ ψ) ⟶ ψ) := by
   eval
   simp [or_assoc, Bool.dichotomy]
+
+theorem conj_comm_t : Tautology ((φ ⋀ ψ) ⟶ (ψ ⋀ φ)) := by
+  eval
+
+theorem conj_comm_t' : Tautology (∼(φ ⋀ ψ) ⟶ ∼(ψ ⋀ φ)) := by
+  simp only [Form.neg, Form.conj]
+  eval
+
+theorem iff_intro : Tautology ((φ ⟶ ψ) ⟶ (ψ ⟶ φ) ⟶ (φ ⟷ ψ)) := by
+  admit
+
+theorem iff_elim_l : Tautology ((φ ⟷ ψ) ⟶ (φ ⟶ ψ)) := by
+  admit
+
+theorem iff_elim_r : Tautology ((φ ⟷ ψ) ⟶ (ψ ⟶ φ)) := by
+  admit
+
+theorem iff_rw : Tautology ((φ ⟷ ψ) ⟶ (ψ ⟷ χ) ⟶ (φ ⟷ χ)) := by
+  admit
+
+theorem iff_imp : Tautology ((φ ⟷ ψ) ⟶ (χ ⟷ τ) ⟶ ((φ ⟶ χ) ⟷ (ψ ⟶ τ))) := by
+  admit
+
+theorem taut_iff_mp : Tautology (φ ⟷ ψ) → Tautology (φ ⟶ ψ) := by
+  rw [Form.iff]
+  intro h e
+  have := h e
+  rw [e_conj] at this
+  exact this.left
+
+theorem taut_iff_mpr : Tautology (φ ⟷ ψ) → Tautology (ψ ⟶ φ) := by
+  rw [Form.iff]
+  intro h e
+  have := h e
+  rw [e_conj] at this
+  exact this.right
 
 theorem disj_intro_l : Tautology (φ ⟶ (φ ⋁ ψ)) := by
   eval
@@ -106,9 +183,18 @@ theorem com12 : Tautology ((φ ⟶ (ψ ⟶ χ)) ⟶ (ψ ⟶ (φ ⟶ χ))) := by
   intro h1 h2 h3
   exact h1 h3 h2
 
-syntax "tautology" : tactic
-macro_rules
-  | `(tactic| tautology) => `(tactic| first | apply dne)
+theorem mp_help : Tautology ((a ⟶ (φ ⟶ ψ)) ⟶ ((b ⟶ φ) ⟶ (a ⟶ b ⟶ ψ))) := by
+  admit
 
 def Eval.nom_variant (e e' : Eval) (i : NOM) (x : SVAR) : Prop :=
   e'.f = (λ φ : Form => if φ = i then (e.f x) else (e.f φ))
+
+theorem iff_not : Tautology ((φ ⟷ ψ) ⟷ (∼φ ⟷ ∼ψ)) := by
+  simp only [Form.iff, Form.conj, Form.neg]
+  eval
+ 
+theorem imp_taut (h : Tautology φ) : Tautology ((φ ⟶ ψ) ⟶ ψ) := by
+  unfold Tautology at h ⊢
+  intro e
+  have := h e
+  simp [this, e.p1, e.p2, e_dn, e_neg, e_conj, e_disj, e_impl, -Form.neg, -Form.conj, -Form.disj, -Form.iff]
